Lean4Lean/Verify/TypeChecker/IsDefEq.lean
@@ -1,0 +1,572 @@
+import Lean4Lean.Verify.TypeChecker.Reduce
+
+namespace Lean4Lean.TypeChecker.Inner
+open Lean hiding Environment Exception
+
+theorem isDefEqLambda.WF {c : VContext} {s : VState}
+    {m} [mwf : c.MLCWF m]
+    {fvs : List Expr} (hsubst : subst.toList.reverse = fvs)
+    (he₁ : (c.withMLC m).TrExprS (e₁.instantiateList fvs) ei₁')
+    (he₂ : (c.withMLC m).TrExprS (e₂.instantiateList fvs) ei₂') :
+    RecM.WF (c.withMLC m) s (isDefEqLambda e₁ e₂ subst) fun b _ =>
+      b → (c.withMLC m).IsDefEqU ei₁' ei₂' := by
+  unfold isDefEqLambda; let c' := c.withMLC m
+  split <;> [rename_i n₁ d₁ b₁ bi₁ n₂ d₂ b₂ bi₂; (simp [hsubst]; exact isDefEq.WF he₁ he₂)]
+  extract_lets F di₁ di₂ G; unfold G di₁ di₂
+  simp at he₁ he₂
+  let .lam (ty' := t₁') (body' := b₁') ⟨_, a1⟩ a2 a3 := he₁
+  let .lam (ty' := t₂') (body' := b₂') b1 b2 b3 := he₂
+  suffices ∀ {x s}
+      (_ : match x with
+        | none => d₁ == d₂
+        | some x => x = d₂.instantiateList fvs),
+      c'.IsDefEqU t₁' t₂' →
+      (F x).WF c' s fun b _ => b → c'.IsDefEqU (t₁'.lam b₁') (t₂'.lam b₂') by
+    split <;> rename_i h
+    · refine .pureBind <| this ‹_› ?_
+      exact a2.eqv (Expr.instantiateList_eqv h) |>.uniq c'.Ewf (.refl c'.Ewf c'.Δwf) b2
+    simp [hsubst]
+    refine (isDefEq.WF a2 b2).bind fun b _ _ h1 => ?_
+    split <;> [exact .pure nofun; rename_i h]
+    simp at h; exact this rfl (h1 h)
+  intros x s hx tt
+  have tt' := tt.of_l c'.Ewf c'.Δwf a1
+  have ⟨b₁'', a3', eq⟩ := a3.defeqDFC' c'.Ewf <| .cons (.refl c'.Ewf c'.Δwf) (by nofun) (.vlam tt')
+  unfold F; split <;> rename_i h
+  · extract_lets d₂'
+    have : d₂' = d₂.instantiateList fvs := by split at hx <;> [simp [d₂', hsubst]; exact hx]
+    clear_value d₂'; subst this
+    refine .withLocalDecl b2 b1 .rfl fun v mwf' _ _ _ => ?_
+    have b3' := b3.inst_fvar c.Ewf mwf'.1.tr.wf
+    have a3'' := a3'.inst_fvar c.Ewf mwf'.1.tr.wf
+    rw [Expr.instantiateList_instantiate1_comm (by rfl), ← Expr.instantiateList] at a3'' b3'
+    refine isDefEqLambda.WF (mwf := mwf') (fvs := .fvar v :: fvs) (by simp [hsubst]) a3'' b3'
+      |>.mono fun _ _ _ h hb => ?_
+    have ⟨_, bb⟩ := eq.symm.trans c'.Ewf mwf'.1.tr.wf.toCtx (h hb)
+    exact ⟨_, .symm <| .lamDF tt'.symm <| bb.symm⟩
+  · simp [Expr.hasLooseBVars] at h
+    refine .stateWF fun wf => ?_
+    have {bᵢ : Expr} {bᵢ'} (h : bᵢ.looseBVarRange' = 0)
+        (a3 : TrExprS c'.venv c'.lparams ((none, .vlam t₂') :: c'.vlctx)
+          (bᵢ.instantiateList fvs 1) bᵢ') :
+        ∃ e', (c.withMLC m).TrExprS (bᵢ.instantiateList (default :: fvs)) e' ∧
+          c'.venv.IsDefEqU c'.lparams.length (t₂' :: c'.vlctx.toCtx) bᵢ' e'.lift := by
+      simp; rw [← Expr.instantiateList_instantiate1_comm (by rfl)]
+      let v : FVarId := ⟨s.ngen.curr⟩
+      have hΔ : VLCtx.WF c'.venv c.lparams.length ((some (v, []), .vlam t₂') :: m.vlctx) := by
+        refine ⟨mwf.1.tr.wf, ?_, b1⟩
+        rintro _ _ ⟨⟩; simp; exact fun h => s.ngen.not_reserves_self (wf.ngen_wf _ h)
+      have := a3.inst_fvar c.Ewf.ordered hΔ
+      have eq {e} (hb : bᵢ.looseBVarRange' = 0) (he : e.looseBVarRange' = 0) :
+          (bᵢ.instantiateList fvs 1).instantiate1' e = bᵢ.instantiateList fvs 1 := by
+        rw [Expr.instantiate1'_eq_self]; rw [Expr.instantiateList'_eq_self] <;> simp [*]
+      rw [eq h rfl, ← eq (e := .fvar v) h rfl]
+      let ⟨_, H⟩ := this.weakFV_inv c.Ewf (.skip_fvar _ _ .refl) (.refl c.Ewf hΔ)
+        (m.noBV ▸ this.closed) (by rw [eq h rfl]; exact a3.fvarsIn)
+      refine ⟨_, H, this.uniq c'.Ewf (.refl c'.Ewf hΔ) <| H.weakFV c'.Ewf (.skip_fvar _ _ .refl) hΔ⟩
+    let ⟨_, a4, a5⟩ := this h.1 a3'
+    let ⟨_, b4, b5⟩ := this h.2 b3
+    exact isDefEqLambda.WF (fvs := default :: fvs) (by simp [hsubst]) a4 b4
+      |>.mono fun _ _ _ h hb =>
+      have hΓ := ⟨c'.Δwf, b1⟩
+      have ⟨_, bb⟩ := eq.symm.trans c'.Ewf hΓ a5
+        |>.trans c'.Ewf hΓ ((h hb).weak c'.Ewf (B := t₂')) |>.trans c'.Ewf hΓ b5.symm
+      ⟨_, .symm <| .lamDF tt'.symm bb.symm⟩
+
+theorem isDefEqForall.WF {c : VContext} {s : VState}
+    {m} [mwf : c.MLCWF m]
+    {fvs : List Expr} (hsubst : subst.toList.reverse = fvs)
+    (he₁ : (c.withMLC m).TrExprS (e₁.instantiateList fvs) ei₁')
+    (he₂ : (c.withMLC m).TrExprS (e₂.instantiateList fvs) ei₂') :
+    RecM.WF (c.withMLC m) s (isDefEqForall e₁ e₂ subst) fun b _ =>
+      b → (c.withMLC m).IsDefEqU ei₁' ei₂' := by
+  unfold isDefEqForall; let c' := c.withMLC m
+  split <;> [rename_i n₁ d₁ b₁ bi₁ n₂ d₂ b₂ bi₂; (simp [hsubst]; exact isDefEq.WF he₁ he₂)]
+  extract_lets F di₁ di₂ G; unfold G di₁ di₂
+  simp at he₁ he₂
+  let .forallE (ty' := t₁') (body' := b₁') ⟨_, a1⟩ _ a2 a3 := he₁
+  let .forallE (ty' := t₂') (body' := b₂') b1 ⟨_, bT⟩ b2 b3 := he₂
+  suffices ∀ {x s}
+      (_ : match x with
+        | none => d₁ == d₂
+        | some x => x = d₂.instantiateList fvs),
+      c'.IsDefEqU t₁' t₂' →
+      (F x).WF c' s fun b _ => b → c'.IsDefEqU (t₁'.forallE b₁') (t₂'.forallE b₂') by
+    split <;> rename_i h
+    · refine .pureBind <| this ‹_› ?_
+      exact a2.eqv (Expr.instantiateList_eqv h) |>.uniq c'.Ewf (.refl c'.Ewf c'.Δwf) b2
+    simp [hsubst]
+    refine (isDefEq.WF a2 b2).bind fun b _ _ h1 => ?_
+    split <;> [exact .pure nofun; rename_i h]
+    simp at h; exact this rfl (h1 h)
+  intros x s hx tt
+  have tt' := tt.of_l c'.Ewf c'.Δwf a1
+  have ⟨b₁'', a3', eq⟩ := a3.defeqDFC' c'.Ewf <| .cons (.refl c'.Ewf c'.Δwf) (by nofun) (.vlam tt')
+  unfold F; split <;> rename_i h
+  · extract_lets d₂'
+    have : d₂' = d₂.instantiateList fvs := by split at hx <;> [simp [d₂', hsubst]; exact hx]
+    clear_value d₂'; subst this
+    refine .withLocalDecl b2 b1 .rfl fun v mwf' _ _ _ => ?_
+    have b3' := b3.inst_fvar c.Ewf mwf'.1.tr.wf
+    have a3'' := a3'.inst_fvar c.Ewf mwf'.1.tr.wf
+    rw [Expr.instantiateList_instantiate1_comm (by rfl), ← Expr.instantiateList] at a3'' b3'
+    refine isDefEqForall.WF (mwf := mwf') (fvs := .fvar v :: fvs) (by simp [hsubst]) a3'' b3'
+      |>.mono fun _ _ _ h hb => ?_
+    have bb := eq.symm.trans c'.Ewf mwf'.1.tr.wf.toCtx (h hb) |>.of_r c'.Ewf mwf'.1.tr.wf.toCtx bT
+    exact ⟨_, .symm <| .forallEDF tt'.symm <| bb.symm⟩
+  · simp [Expr.hasLooseBVars] at h
+    refine .stateWF fun wf => ?_
+    have {bᵢ : Expr} {bᵢ'} (h : bᵢ.looseBVarRange' = 0)
+        (a3 : TrExprS c'.venv c'.lparams ((none, .vlam t₂') :: c'.vlctx)
+          (bᵢ.instantiateList fvs 1) bᵢ') :
+        ∃ e', (c.withMLC m).TrExprS (bᵢ.instantiateList (default :: fvs)) e' ∧
+          c'.venv.IsDefEqU c'.lparams.length (t₂' :: c'.vlctx.toCtx) bᵢ' e'.lift := by
+      simp; rw [← Expr.instantiateList_instantiate1_comm (by rfl)]
+      let v : FVarId := ⟨s.ngen.curr⟩
+      have hΔ : VLCtx.WF c'.venv c.lparams.length ((some (v, []), .vlam t₂') :: m.vlctx) := by
+        refine ⟨mwf.1.tr.wf, ?_, b1⟩
+        rintro _ _ ⟨⟩; simp; exact fun h => s.ngen.not_reserves_self (wf.ngen_wf _ h)
+      have := a3.inst_fvar c.Ewf.ordered hΔ
+      have eq {e} (hb : bᵢ.looseBVarRange' = 0) (he : e.looseBVarRange' = 0) :
+          (bᵢ.instantiateList fvs 1).instantiate1' e = bᵢ.instantiateList fvs 1 := by
+        rw [Expr.instantiate1'_eq_self]; rw [Expr.instantiateList'_eq_self] <;> simp [*]
+      rw [eq h rfl, ← eq (e := .fvar v) h rfl]
+      let ⟨_, H⟩ := this.weakFV_inv c.Ewf (.skip_fvar _ _ .refl) (.refl c.Ewf hΔ)
+        (m.noBV ▸ this.closed) (by rw [eq h rfl]; exact a3.fvarsIn)
+      refine ⟨_, H, this.uniq c'.Ewf (.refl c'.Ewf hΔ) <| H.weakFV c'.Ewf (.skip_fvar _ _ .refl) hΔ⟩
+    let ⟨_, a4, a5⟩ := this h.1 a3'
+    let ⟨_, b4, b5⟩ := this h.2 b3
+    exact isDefEqForall.WF (fvs := default :: fvs) (by simp [hsubst]) a4 b4
+      |>.mono fun _ _ _ h hb =>
+      have hΓ := ⟨c'.Δwf, b1⟩
+      have bb := eq.symm.trans c'.Ewf hΓ a5 |>.trans c'.Ewf hΓ ((h hb).weak c'.Ewf (B := t₂'))
+        |>.trans c'.Ewf hΓ b5.symm |>.of_r c'.Ewf hΓ bT
+      ⟨_, .symm <| .forallEDF tt'.symm bb.symm⟩
+
+theorem EquivManager.isEquiv.WF {c : VContext}
+    (he₁ : c.TrExprS e₁ e₁') (he₂ : c.TrExprS e₂ e₂')
+    (H : EquivManager.isEquiv useHash e₁ e₂ m = (b, m')) :
+    b → c.IsDefEqU e₁' e₂' := by
+  sorry
+
+theorem quickIsDefEq.WF {c : VContext} {s : VState}
+    (he₁ : c.TrExprS e₁ e₁') (he₂ : c.TrExprS e₂ e₂') :
+    RecM.WF c s (quickIsDefEq e₁ e₂ useHash) fun b _ => b = .true → c.IsDefEqU e₁' e₂' := by
+  unfold quickIsDefEq
+  refine .bind (Q := fun b _ => b = true → c.IsDefEqU e₁' e₂') ?_ fun _ _ _ h => ?_
+  · intro _ mwf wf _ s₁ eq
+    simp [modifyGet, MonadStateOf.modifyGet, monadLift, MonadLift.monadLift, StateT.modifyGet,
+      pure, Except.pure] at eq
+    split at eq; rename_i b _ b' m hm
+    change let s' := _; (_, s') = _ at eq; extract_lets s' at eq
+    injection eq; subst b' s₁
+    have h1 := EquivManager.isEquiv.WF he₁ he₂ hm
+    exact let vs' := { s with toState := s' }; ⟨vs', rfl, .rfl, { wf with }, h1⟩
+  extract_lets F; split <;> [exact .pure fun _ => h ‹_›; skip]
+  refine .pureBind ?_; unfold F; split
+  · exact .toLBoolM <| c.withMLC_self ▸
+      isDefEqLambda.WF (subst := #[]) (fvs := []) rfl (c.withMLC_self ▸ he₁) (c.withMLC_self ▸ he₂)
+  · exact .toLBoolM <| c.withMLC_self ▸
+      isDefEqForall.WF (subst := #[]) (fvs := []) rfl (c.withMLC_self ▸ he₁) (c.withMLC_self ▸ he₂)
+  · have .sort hu := he₁; have .sort hv := he₂
+    refine .pure fun h => ⟨_, .sortDF (.of_ofLevel hu) (.of_ofLevel hv) ?_⟩
+    exact Level.isEquiv'_wf (toLBool_true.1 h) hu hv
+  · let .mdata he₁ := he₁; let .mdata he₂ := he₂
+    exact .toLBoolM <| isDefEq.WF he₁ he₂
+  · cases he₁
+  · rename_i a1 a2 _; refine .pure fun h => ?_
+    simp at h; subst h; exact he₁.uniq c.Ewf (.refl c.Ewf c.Δwf) he₂
+  · exact .pure nofun
+
+theorem isDefEqArgs.WF {c : VContext} {s : VState}
+    (H : ∃ e₁', c.TrExprS e₁.getAppFn e₁' ∧ ∃ e₂', c.TrExprS e₂.getAppFn e₂' ∧ c.IsDefEqU e₁' e₂')
+    (he₁ : c.TrExprS e₁ e₁') (he₂ : c.TrExprS e₂ e₂') :
+    RecM.WF c s (isDefEqArgs e₁ e₂) fun b _ => b → c.IsDefEqU e₁' e₂' := by
+  unfold isDefEqArgs; split <;> (unfold Expr.getAppFn at H)
+  · let .app a1 a2 a3 a4 := he₁
+    let .app b1 b2 b3 b4 := he₂
+    refine (isDefEq.WF a4 b4).bind fun _ _ _ h2 => ?_; extract_lets F
+    split <;> [exact .pure nofun; rename_i hb2]
+    refine (isDefEqArgs.WF H a3 b3).mono fun _ _ _ h1 hb1 => ?_
+    simp at hb2
+    exact ⟨_, .appDF ((h1 hb1).of_l c.Ewf c.Δwf a1) ((h2 hb2).of_l c.Ewf c.Δwf a2)⟩
+  · exact .pure nofun
+  · exact .pure nofun
+  · refine .pure fun _ => ?_
+    simp [*] at H; let ⟨_, h1, _, h2, h3⟩ := H
+    have a1 := he₁.uniq c.Ewf (.refl c.Ewf c.Δwf) h1
+    have a2 := he₂.uniq c.Ewf (.refl c.Ewf c.Δwf) h2
+    exact a1.trans c.Ewf c.Δwf h3 |>.trans c.Ewf c.Δwf a2.symm
+
+theorem tryEtaExpansionCore.WF {c : VContext} {s : VState}
+    (he₁ : c.TrExprS e₁ e₁') (he₂ : c.TrExprS e₂ e₂') :
+    RecM.WF c s (tryEtaExpansionCore e₁ e₂) fun b _ => b → c.IsDefEqU e₁' e₂' := by
+  unfold tryEtaExpansionCore; split <;> [skip; exact .pure nofun]
+  refine (inferType.WF he₂).bind fun _ _ _ ⟨ty₁, a1, a2, a3, a4⟩ => ?_
+  refine (whnf.WF a3).bind fun _ _ _ ⟨b1, _, b2, b3⟩ => ?_
+  split <;> [skip; exact .pure nofun]
+  let .forallE (ty' := ty') c1 c2 c3 c4 := b2
+  replace a4 := a4.defeqU_r c.Ewf c.Δwf b3.symm
+  -- have := b2.uniq c.Ewf (.refl c.Ewf c.Δwf) (.forallE c1 c2 c3 c4)
+  refine (isDefEq.WF he₁ (.lam c1 c3 (.app (a4.weak c.Ewf) (.bvar .zero) (
+    Expr.liftLooseBVars_eq_self (c.mlctx.noBV ▸ a2.closed).looseBVarRange_le ▸
+      a2.weakBV c.Ewf (.skip (.vlam ty') .refl)) (.bvar rfl)))).mono fun _ _ _ h hb => ?_
+  exact (h hb).trans c.Ewf c.Δwf ⟨_, .eta a4⟩
+
+theorem tryEtaExpansion.WF {c : VContext} {s : VState}
+    (he₁ : c.TrExprS e₁ e₁') (he₂ : c.TrExprS e₂ e₂') :
+    RecM.WF c s (tryEtaExpansion e₁ e₂) fun b _ => b → c.IsDefEqU e₁' e₂' := by
+  simp [tryEtaExpansion, orM, toBool]
+  refine (tryEtaExpansionCore.WF he₁ he₂).bind fun _ _ _ h => ?_
+  split <;> [exact .pure fun _ => h rfl; skip]
+  exact (tryEtaExpansionCore.WF he₂ he₁).mono fun _ _ _ h hb => (h hb).symm
+
+theorem tryEtaStructCore.WF {c : VContext} {s : VState}
+    (he₁ : c.TrExprS e₁ e₁') (he₂ : c.TrExprS e₂ e₂') :
+    RecM.WF c s (tryEtaStructCore e₁ e₂) fun b _ => b → c.IsDefEqU e₁' e₂' := sorry
+
+theorem tryEtaStruct.WF {c : VContext} {s : VState}
+    (he₁ : c.TrExprS e₁ e₁') (he₂ : c.TrExprS e₂ e₂') :
+    RecM.WF c s (tryEtaStruct e₁ e₂) fun b _ => b → c.IsDefEqU e₁' e₂' := by
+  simp [tryEtaStruct, orM, toBool]
+  refine (tryEtaStructCore.WF he₁ he₂).bind fun _ _ _ h => ?_
+  split <;> [exact .pure fun _ => h rfl; skip]
+  exact (tryEtaStructCore.WF he₂ he₁).mono fun _ _ _ h hb => (h hb).symm
+
+theorem isDefEqApp.WF {c : VContext} {s : VState}
+    (he₁ : c.TrExprS e₁ e₁') (he₂ : c.TrExprS e₂ e₂') :
+    RecM.WF c s (isDefEqApp e₁ e₂) fun b _ => b → c.IsDefEqU e₁' e₂' := by
+  unfold isDefEqApp; extract_lets F1
+  split <;> [(refine .pureBind ?_; unfold F1); exact .pure nofun]
+  rw [Expr.withApp_eq, Expr.withApp_eq]
+  split <;> [rename_i eq; exact .pure nofun]
+  have ⟨_, he₁'⟩ := AppStack.build <| e₁.mkAppList_getAppArgsList ▸ he₁
+  have ⟨_, he₂'⟩ := AppStack.build <| e₂.mkAppList_getAppArgsList ▸ he₂
+  refine (isDefEq.WF he₁'.tr he₂'.tr).bind fun _ _ _ h => ?_; extract_lets F2
+  split <;> [(refine .pureBind ?_; unfold F2); exact .pure nofun]
+  let rec loop.WF {s args₁ args₂ f₁ f₂ f₁' f₂' eq i} (l₁ r₁ l₂ r₂)
+      (h₁ : args₁.toList = l₁ ++ r₁) (hi₁ : l₁.length = i)
+      (h₂ : args₂.toList = l₂ ++ r₂) (hi₂ : l₂.length = i)
+      (he₁ : AppStack c.venv c.lparams c.vlctx (.mkAppList f₁ l₁) f₁' r₁)
+      (he₂ : AppStack c.venv c.lparams c.vlctx (.mkAppList f₂ l₂) f₂' r₂)
+      (H1 : c.IsDefEqU f₁' f₂') :
+      RecM.WF c s (loop args₁ args₂ eq i) fun b _ => b →
+        ∀ e₁', c.TrExprS (f₁.mkAppList args₁.toList) e₁' →
+        ∀ e₂', c.TrExprS (f₂.mkAppList args₂.toList) e₂' → c.IsDefEqU e₁' e₂' := by
+    unfold loop; split <;> rename_i h
+    · have hr₁ : r₁.length > 0 := by simp [← Array.length_toList, h₁] at h; omega
+      have hr₂ : r₂.length > 0 := by simp [eq, ← Array.length_toList, h₂] at h; omega
+      let .app (a := a₁) (as := r₁) a1 a2 a3 a4 a5 := he₁
+      let .app (a := a₂) (as := r₂) b1 b2 b3 b4 b5 := he₂
+      simp [
+        show args₁[i] = a₁ by cases args₁; cases h₁; simp [hi₁],
+        show args₂[i] = a₂ by cases args₂; cases h₂; simp [hi₂]]
+      refine (isDefEq.WF a4 b4).bind fun _ _ _ h => ?_
+      split <;> [skip; exact .pure nofun]
+      have H := (H1.of_l c.Ewf c.Δwf a1).appDF <| (h ‹_›).of_l c.Ewf c.Δwf a2
+      exact loop.WF (l₁ ++ [a₁]) r₁ (l₂ ++ [a₂]) r₂
+        (by simp [h₁]) (by simp [hi₁]) (by simp [h₂]) (by simp [hi₂])
+        (by simp [a5]) (by simp [b5]) ⟨_, H⟩
+    · have hr₁ : r₁.length = 0 := by simp [← Array.length_toList, h₁] at h; omega
+      have hr₂ : r₂.length = 0 := by simp [eq, ← Array.length_toList, h₂] at h; omega
+      simp at hr₁ hr₂; subst r₁ r₂; simp at h₁ h₂; subst l₁ l₂
+      refine .pure fun _ _ h1 _ h2 => ?_
+      have u1 := h1.uniq c.Ewf (.refl c.Ewf c.Δwf) he₁.tr
+      have u2 := h2.uniq c.Ewf (.refl c.Ewf c.Δwf) he₂.tr
+      exact u1.trans c.Ewf c.Δwf H1 |>.trans c.Ewf c.Δwf u2.symm
+  refine loop.WF [] _ [] _ (i := 0) (by simp [Expr.getAppArgs_toList]) rfl
+    (by simp [Expr.getAppArgs_toList]) rfl he₁' he₂' (h ‹_›) |>.mono fun _ _ _ h2 hb => ?_
+  simp [Expr.getAppArgs_toList, Expr.mkAppList_getAppArgsList] at h2
+  exact h2 hb _ he₁ _ he₂
+
+theorem isProp.WF
+    (he : c.TrExprS e e') : (isProp e).WF c s fun b _ => b → c.HasType e' (.sort .zero) := by
+  unfold isProp
+  refine (inferType.WF he).bind fun ty _ le ⟨ty', _, _, h1, h2⟩ => ?_
+  refine .stateWF fun wf => ?_
+  refine (whnf.WF h1).bind fun ty _ le ⟨_, ty₂, h3, h4⟩ => .pure ?_
+  simp [Expr.prop, Expr.eqv_sort]; rintro rfl
+  let .sort h3 := h3; cases h3
+  exact h2.defeqU_r c.Ewf c.Δwf h4.symm
+
+theorem isDefEqProofIrrel.WF {c : VContext} {s : VState}
+    (he₁ : c.TrExprS e₁ e₁') (he₂ : c.TrExprS e₂ e₂') :
+    RecM.WF c s (isDefEqProofIrrel e₁ e₂) fun b _ => b = .true → c.IsDefEqU e₁' e₂' := by
+  unfold isDefEqProofIrrel
+  refine (inferType.WF he₁).bind fun _ _ _ ⟨_, a1, a2, a3, a4⟩ => ?_; extract_lets F1
+  refine (isProp.WF a3).bind fun _ _ _ h1 => ?_
+  split <;> [exact .pure nofun; (refine .pureBind ?_; unfold F1)]
+  rename_i h; simp at h
+  refine (inferType.WF he₂).bind fun _ _ _ ⟨_, b1, b2, b3, b4⟩ => .toLBoolM ?_
+  refine (isDefEq.WF a3 b3).mono fun _ _ _ h2 hb => ?_
+  exact ⟨_, .proofIrrel (h1 h) a4 (b4.defeqU_r c.Ewf c.Δwf (h2 hb).symm)⟩
+
+theorem cacheFailure.WF {c : VContext} {s : VState} :
+    (cacheFailure e₁ e₂).WF c s fun _ _ => True := by
+  rintro wf _ _ ⟨⟩
+  exact ⟨{ s with toState := _ }, rfl, .rfl, { wf with }, ⟨⟩⟩
+
+theorem tryUnfoldProjApp.WF {c : VContext} {s : VState} (he : c.TrExprS e e') :
+    (tryUnfoldProjApp e).WF c s fun oe _ =>
+    ∀ e₁, oe = some e₁ → c.FVarsBelow e e₁ ∧ c.TrExpr e₁ e' := by
+  unfold tryUnfoldProjApp; extract_lets f F
+  split <;> [exact .pure nofun; skip]
+  refine .pureBind ?_; unfold F
+  refine (whnfCore.WF he).bind fun _ _ _ h => ?_
+  refine .pure fun _ => ?_
+  split <;> rintro ⟨⟩; exact h
+
+def _root_.Lean4Lean.TypeChecker.ReductionStatus.WF
+    (c : VContext) (e₁' e₂' : VExpr) (allowContinue := false) : ReductionStatus → Prop
+  | .continue e₁ e₂ => allowContinue ∧ c.TrExpr e₁ e₁' ∧ c.TrExpr e₂ e₂'
+  | .unknown e₁ e₂ => c.TrExpr e₁ e₁' ∧ c.TrExpr e₂ e₂'
+  | .bool b => b → c.IsDefEqU e₁' e₂'
+
+def _root_.Lean4Lean.TypeChecker.ReductionStatus.WF.defeq
+    (h1 : c.IsDefEqU e₁' e₁'') (h2 : c.IsDefEqU e₂' e₂'')
+    (H : ReductionStatus.WF c e₁' e₂' ac r) : ReductionStatus.WF c e₁'' e₂'' ac r :=
+  match r, H with
+  | .continue .., ⟨a1, a2, a3⟩ =>
+    ⟨a1, a2.defeq c.Ewf c.Δwf h1, a3.defeq c.Ewf c.Δwf h2⟩
+  | .unknown .., ⟨a2, a3⟩ =>
+    ⟨a2.defeq c.Ewf c.Δwf h1, a3.defeq c.Ewf c.Δwf h2⟩
+  | .bool _, h => fun hb => h1.symm.trans c.Ewf c.Δwf (h hb) |>.trans c.Ewf c.Δwf h2
+
+theorem unfoldDefinitionCore_is_some
+    (h1 : env.find? n = some ci) (h2 : ci.value? = some v) (h3 : ls.length = ci.numLevelParams) :
+    ∃ e₁, unfoldDefinitionCore env (.const n ls) = some e₁ := by
+  simp [unfoldDefinitionCore]
+  rw [isDelta_is_some.2 ⟨_, h1, ⟨_, h2⟩, _, rfl⟩]; simp [h3]
+
+theorem unfoldDefinition_is_some (h1 : env.find? n = some ci) (h2 : ci.value? = some v)
+    (h3 : e.getAppFn = .const n ls) (h4 : ls.length = ci.numLevelParams) :
+    ∃ e₁, unfoldDefinition env e = some e₁ := by
+  simp [unfoldDefinition]; revert h3; unfold Expr.getAppFn Expr.isApp; split
+  · rename_i f a
+    intro e; simp [e]
+    exact let ⟨_, h⟩ := unfoldDefinitionCore_is_some h1 h2 h4; h ▸ ⟨_, rfl⟩
+  · rintro rfl; exact unfoldDefinitionCore_is_some h1 h2 h4
+
+theorem lazyDeltaReductionStep.WF {c : VContext} {s : VState}
+    (he₁ : c.TrExprS e₁ e₁') (he₂ : c.TrExprS e₂ e₂') :
+    (lazyDeltaReductionStep e₁ e₂).WF c s fun r _ => r.WF c e₁' e₂' true := by
+  unfold lazyDeltaReductionStep
+  refine .getEnv ?_; extract_lets delta cont F1 F2
+  have hdelta {s e e' ci} (he : c.TrExprS e e') (H : isDelta c.env e = some ci) :
+      (delta e).WF c s fun r _ => c.TrExpr r e' := by
+    let ⟨n, h1, ⟨_, h2⟩, ls, h3⟩ := isDelta_is_some.1 H
+    have ⟨_, stk⟩ := AppStack.build (e.mkAppList_getAppArgsList ▸ he)
+    have .const a1 a2 a3 := h3 ▸ stk.tr
+    have ⟨b1, b2, b3, b4⟩ := c.trenv.find?_uniq h1 a1
+    let ⟨_, h⟩ := unfoldDefinition_is_some h1 h2 h3 (a3.trans b3.symm)
+    simp [delta, h]
+    have ⟨_, _, c1, c2⟩ := unfoldDefinition.WF he h
+    exact (whnfCore.WF c1).mono fun x _ _ h => h.2.defeq c.Ewf c.Δwf c2
+  have hcont {s e₁ e₂} (he₁ : c.TrExpr e₁ e₁') (he₂ : c.TrExpr e₂ e₂') :
+      (cont e₁ e₂).WF c s fun r _ => r.WF c e₁' e₂' true := by
+    let ⟨_, se₁, de₁⟩ := he₁; let ⟨_, se₂, de₂⟩ := he₂
+    refine (quickIsDefEq.WF se₁ se₂).bind fun _ _ _ h => .pure ?_; split
+    · exact ⟨rfl, he₁, he₂⟩
+    · intro; exact de₁.symm.trans c.Ewf c.Δwf (h rfl) |>.trans c.Ewf c.Δwf de₂
+    · nofun
+  split
+  · exact .pure ⟨he₁.trExpr c.Ewf c.Δwf, he₂.trExpr c.Ewf c.Δwf⟩
+  · refine (tryUnfoldProjApp.WF he₂).bind fun _ _ _ h => ?_; split
+    · exact hcont (he₁.trExpr c.Ewf c.Δwf) (h _ rfl).2
+    · exact (hdelta he₁ ‹_›).bind fun _ _ _ h => hcont h (he₂.trExpr c.Ewf c.Δwf)
+  · refine (tryUnfoldProjApp.WF he₁).bind fun _ _ _ h => ?_; split
+    · exact hcont (h _ rfl).2 (he₂.trExpr c.Ewf c.Δwf)
+    · exact (hdelta he₂ ‹_›).bind fun _ _ _ h => hcont (he₁.trExpr c.Ewf c.Δwf) h
+  rename_i dt dt' hd1 hd2; extract_lets ht hs; split <;> [skip; split]
+  · exact (hdelta he₂ ‹_›).bind fun _ _ _ h => hcont (he₁.trExpr c.Ewf c.Δwf) h
+  · exact (hdelta he₁ ‹_›).bind fun _ _ _ h => hcont h (he₂.trExpr c.Ewf c.Δwf)
+  have hF1 {s} : (F1 ⟨⟩).WF c s fun r _ => r.WF c e₁' e₂' true :=
+    (hdelta he₁ ‹_›).bind fun _ _ _ h1 => (hdelta he₂ ‹_›).bind fun _ _ _ h2 => hcont h1 h2
+  refine .get ?_; split <;> [skip; exact hF1]
+  split <;> [skip; exact cacheFailure.WF.lift.bind fun _ _ _ _ => hF1]
+  rename_i h1 h2; simp at h1
+  cases ptrEqConstantInfo_eq h1.1.1.2
+  have ⟨n₁, b1₁, ⟨_, b2₁⟩, ls₁, b3₁⟩ := isDelta_is_some.1 hd1
+  have ⟨n₂, b1₂, ⟨_, b2₂⟩, ls₂, b3₂⟩ := isDelta_is_some.1 hd2
+  simp [b3₁, b3₂, Expr.constLevels!] at h2
+  have ⟨_, stk₁⟩ := AppStack.build (e₁.mkAppList_getAppArgsList ▸ he₁)
+  have ⟨_, stk₂⟩ := AppStack.build (e₂.mkAppList_getAppArgsList ▸ he₂)
+  have .const (us' := ls₁) c1₁ c2₁ c3₁ := b3₁ ▸ stk₁.tr
+  have .const (us' := ls₂) c1₂ c2₂ c3₂ := b3₂ ▸ stk₂.tr
+  cases (c.trenv.find?_uniq b1₁ c1₁).1
+  cases (c.trenv.find?_uniq b1₂ c1₂).1
+  cases c1₁.symm.trans c1₂
+  have := VEnv.IsDefEq.constDF c1₁
+    (Γ := c.vlctx.toCtx) (.of_mapM_ofLevel c2₁) (.of_mapM_ofLevel c2₂)
+    ((List.mapM_eq_some.1 c2₁).length_eq.symm.trans c3₁)
+    (Level.isEquivList_wf h2 c2₁ c2₂)
+  refine (isDefEqArgs.WF ⟨_, stk₁.tr, _, stk₂.tr, _, this⟩ he₁ he₂).bind fun _ _ _ h => ?_
+  split <;> [skip; exact cacheFailure.WF.lift.bind fun _ _ _ _ => hF1]
+  exact .pure fun _ => h ‹_›
+
+theorem isNatZero_wf {c : VContext} (H : isNatZero e) (h : c.TrExprS e e') : e' = .natZero := by
+  have h1 : c.TrExprS (.lit (.natVal 0)) e' := by
+    simp [isNatZero] at H; obtain H|H := H
+    · exact .lit (h.eqv H)
+    · split at H <;> [exact h; cases H]
+  have := TrExprS.lit_has_type c.Ewf c.hasPrimitives (l := .natVal 0) h1
+  exact h1.unique (by trivial) (TrExprS.natLit c.hasPrimitives this 0).1
+
+theorem isNatSuccOf?_wf {c : VContext} (H : isNatSuccOf? e = some e₁)
+    (h : c.TrExprS e e') : ∃ x, c.TrExprS e₁ x ∧ e' = .app .natSucc x := by
+  unfold isNatSuccOf? at H; split at H <;> cases H
+  · rename_i n
+    have := TrExprS.lit_has_type c.Ewf c.hasPrimitives (l := .natVal (n+1)) h
+    refine ⟨_, (TrExprS.natLit c.hasPrimitives this n).1, ?_⟩
+    exact h.unique (by trivial) (TrExprS.natLit c.hasPrimitives this (n+1)).1
+  · let .app a1 a2 a3 a4 := h
+    let .const b1 b2 b3 := a3
+    cases c.hasPrimitives.natSucc b1
+    simp at b3; subst b3; simp at b2; subst b2
+    exact ⟨_, a4, rfl⟩
+
+theorem isDefEqOffset.WF {c : VContext} {s : VState}
+    (he₁ : c.TrExprS e₁ e₁') (he₂ : c.TrExprS e₂ e₂') :
+    (isDefEqOffset e₁ e₂).WF c s fun b _ => b = .true → c.IsDefEqU e₁' e₂' := by
+  unfold isDefEqOffset; extract_lets F; split
+  · rename_i h; simp at h
+    cases isNatZero_wf h.1 he₁; cases isNatZero_wf h.2 he₂
+    exact .pure fun _ => .refl <| he₁.wf c.Ewf c.Δwf
+  · refine .pureBind ?_; unfold F; split <;> [skip; exact .pure nofun]
+    obtain ⟨_, a1, rfl⟩ := isNatSuccOf?_wf ‹_› he₁
+    obtain ⟨_, b1, rfl⟩ := isNatSuccOf?_wf ‹_› he₂
+    refine .toLBoolM <| (isDefEqCore.WF a1 b1).mono fun _ _ _ h hb => ?_
+    let ⟨_, de'⟩ := he₁.wf c.Ewf c.Δwf
+    let ⟨_, _, c1, c2⟩ := de'.hasType.1.app_inv c.Ewf c.Δwf
+    exact ⟨_, c1.appDF <| (h hb).of_l c.Ewf c.Δwf c2⟩
+
+theorem lazyDeltaReduction.loop.WF {c : VContext} {s : VState}
+    (he₁ : c.TrExprS e₁ e₁') (he₂ : c.TrExprS e₂ e₂') :
+    (lazyDeltaReduction.loop e₁ e₂ n).WF c s fun r _ => r.WF c e₁' e₂' := by
+  induction n generalizing s e₁ e₂ e₁' e₂' with | zero => exact .throw | succ n ih
+  unfold loop; extract_lets F1 F2 F3
+  refine (isDefEqOffset.WF he₁ he₂).bind fun _ _ _ h => ?_; split
+  · exact .pure fun hb => h (by simpa using hb)
+  suffices hF2 : ∀ {s}, (F2 ⟨⟩).WF c s fun r _ => r.WF c e₁' e₂' by
+    refine .pureBind <|.readThe ?_; split <;> [skip; exact hF2]
+    refine (reduceNat.WF he₁).bind fun _ _ _ h => ?_; split
+    · have ⟨_, a1, a2⟩ := (h _ rfl).2
+      refine (isDefEqCore.WF a1 he₂).bind fun _ _ _ h => .pure fun hb => ?_
+      exact a2.symm.trans c.Ewf c.Δwf (h hb)
+    refine (reduceNat.WF he₂).bind fun _ _ _ h => ?_; split
+    · have ⟨_, a1, a2⟩ := (h _ rfl).2
+      refine (isDefEqCore.WF he₁ a1).bind fun _ _ _ h => .pure fun hb => ?_
+      exact (h hb).trans c.Ewf c.Δwf a2
+    exact hF2
+  intro s; unfold F2; refine .getEnv ?_
+  refine (M.WF.liftExcept reduceNative.WF).lift.bind fun _ _ _ h => ?_
+  split <;> [cases h _ rfl; skip]
+  refine (M.WF.liftExcept reduceNative.WF).lift.bind fun _ _ _ h => ?_
+  split <;> [cases h _ rfl; skip]
+  refine .pureBind ?_; unfold F1
+  refine (lazyDeltaReductionStep.WF he₁ he₂).bind fun r _ _ h => ?_
+  obtain r|r|r := r
+  · let ⟨_, ⟨_, a1, a2⟩, ⟨_, b1, b2⟩⟩ := h
+    exact (ih a1 b1).mono fun _ _ _ h => h.defeq a2 b2
+  · exact .pure h
+  · exact .pure h
+
+theorem tryStringLitExpansionCore.WF {c : VContext} {s : VState}
+    (he₁ : c.TrExprS e₁ e₁') (he₂ : c.TrExprS e₂ e₂') :
+    RecM.WF c s (tryStringLitExpansionCore e₁ e₂) fun b _ => b = .true → c.IsDefEqU e₁' e₂' := by
+  unfold tryStringLitExpansionCore; iterate 3 split <;> [skip; exact .pure nofun]
+  let .lit he₁ := he₁
+  exact .toLBoolM <| isDefEqCore.WF he₁ he₂
+
+theorem tryStringLitExpansion.WF {c : VContext} {s : VState}
+    (he₁ : c.TrExprS e₁ e₁') (he₂ : c.TrExprS e₂ e₂') :
+    RecM.WF c s (tryStringLitExpansion e₁ e₂) fun b _ => b = .true → c.IsDefEqU e₁' e₂' := by
+  refine (tryStringLitExpansionCore.WF he₁ he₂).bind fun _ _ _ h => ?_
+  split <;> [skip; exact .pure h]
+  exact (tryStringLitExpansionCore.WF he₂ he₁).mono fun _ _ _ h hb => (h hb).symm
+
+theorem isDefEqUnitLike.WF {c : VContext} {s : VState}
+    (he₁ : c.TrExprS e₁ e₁') (he₂ : c.TrExprS e₂ e₂') :
+    RecM.WF c s (isDefEqUnitLike e₁ e₂) fun b _ => b = .true → c.IsDefEqU e₁' e₂' := sorry
+
+theorem isDefEqCore'.WF {c : VContext} {s : VState}
+    (he₁ : c.TrExprS e₁ e₁') (he₂ : c.TrExprS e₂ e₂') :
+    RecM.WF c s (isDefEqCore' e₁ e₂) fun b _ => b = true → c.IsDefEqU e₁' e₂' := by
+  unfold isDefEqCore'; extract_lets F1 F2 F3
+  refine (quickIsDefEq.WF he₁ he₂).bind fun _ _ _ h => ?_
+  split <;> [exact .pure fun hb => h (by simpa using hb); skip]
+  refine .pureBind <| .readThe ?_
+  suffices ∀ {s}, RecM.WF c s (F2 ⟨⟩) fun b _ => b = true → c.IsDefEqU e₁' e₂' by
+    split <;> [rename_i h1; exact this]
+    refine (whnf.WF he₁).bind fun _ _ _ ⟨_, _, a1, a2⟩ => ?_
+    split <;> [rename_i h2; exact this]
+    refine .pure fun _ => ?_
+    simp [Expr.isConstOf] at h1 h2
+    split at h1 <;> simp at h1; cases h1.2; split at h2 <;> simp at h2; cases h2
+    let .const b1 b2 b3 := he₂
+    let .const c1 c2 c3 := a1
+    cases c.hasPrimitives.boolTrue b1
+    cases c.hasPrimitives.boolTrue c1
+    simp at b3 c3; subst b3 c3; simp at b2 c2; subst b2 c2
+    exact a2.symm
+  intro; unfold F2
+  refine (whnfCore.WF he₁).bind fun _ _ _ ⟨_, e₁', a1, a2⟩ => ?_
+  refine (whnfCore.WF he₂).bind fun _ _ _ ⟨_, e₂', b1, b2⟩ => ?_
+  extract_lets F2 F3
+  refine .mono (Q := fun b _ => b = true → c.IsDefEqU e₁' e₂') ?_ fun _ _ _ h hb =>
+    a2.symm.trans c.Ewf c.Δwf (h (by simpa using hb)) |>.trans c.Ewf c.Δwf b2
+  suffices ∀ {s}, RecM.WF c s (F3 ⟨⟩) fun b _ => b = true → c.IsDefEqU e₁' e₂' by
+    split <;> [skip; exact this]
+    refine (quickIsDefEq.WF a1 b1).bind fun _ _ _ h => ?_
+    split <;> [skip; exact this]
+    exact .pure fun hb => h (by simpa using hb)
+  intro; unfold F3
+  refine (isDefEqProofIrrel.WF a1 b1).bind fun _ _ _ h => ?_
+  split
+  · exact .pure fun hb => h (by simpa using hb)
+  refine .pureBind <| (lazyDeltaReduction.loop.WF a1 b1).bind fun _ _ _ h => ?_; split
+  · cases h.1
+  · exact .pure h
+  have ⟨⟨e₁', c1, c4⟩, ⟨e₂', d1, d4⟩⟩ := h
+  refine .mono (Q := fun b _ => b = true → c.IsDefEqU e₁' e₂') ?_ fun _ _ _ h hb =>
+    c4.symm.trans c.Ewf c.Δwf (h (by simpa using hb)) |>.trans c.Ewf c.Δwf d4
+  extract_lets F2 F3 F4 F5 F6 F7
+  suffices ∀ {s}, RecM.WF c s (F7 ⟨⟩) fun b _ => b = true → c.IsDefEqU e₁' e₂' by
+    split
+    · split <;> [rename_i h2; exact this]
+      refine .pure fun _ => ?_
+      simp at h2; cases h2.1
+      have .const c1 c2 c3 := c1; have .const d1 d2 d3 := d1
+      cases d1.symm.trans c1
+      have := VEnv.IsDefEq.constDF c1
+        (Γ := c.vlctx.toCtx) (.of_mapM_ofLevel c2) (.of_mapM_ofLevel d2)
+        ((List.mapM_eq_some.1 c2).length_eq.symm.trans c3)
+        (Level.isEquivList_wf h2.2 c2 d2)
+      exact this.toU
+    · split <;> [rename_i h; exact this]
+      simp at h; subst h
+      exact .pure fun _ => c1.uniq c.Ewf (.refl c.Ewf c.Δwf) d1
+    · split <;> [rename_i h2; exact this]
+      have .proj c1 c2 := c1; have .proj d1 d2 := d1
+      refine (isDefEq.WF c1 d1).bind fun _ _ _ h => ?_
+      split <;> [skip; exact this]
+      refine .pure fun _ => ?_
+      sorry -- proj
+    · exact this
+  intro; unfold F7
+  refine (whnfCore.WF c1).bind fun _ _ _ ⟨_, e₁'', c5, c6⟩ => ?_
+  refine (whnfCore.WF d1).bind fun _ _ _ ⟨_, e₂'', d5, d6⟩ => ?_
+  split
+  · exact (isDefEqCore.WF c5 d5).bind fun _ _ _ h => .pure fun hb =>
+      c6.symm.trans c.Ewf c.Δwf (h (by simpa using hb)) |>.trans c.Ewf c.Δwf d6
+  refine .pureBind <| (isDefEqApp.WF c1 d1).bind fun _ _ _ h => ?_
+  split <;> [exact .pure fun _ => h ‹_›; skip]
+  refine .pureBind <| (tryEtaExpansion.WF c1 d1).bind fun _ _ _ h => ?_
+  split <;> [exact .pure fun _ => h ‹_›; skip]
+  refine .pureBind <| (tryEtaStruct.WF c1 d1).bind fun _ _ _ h => ?_
+  split <;> [exact .pure fun _ => h ‹_›; skip]
+  refine .pureBind <| (tryStringLitExpansion.WF c1 d1).bind fun _ _ _ h => ?_
+  split <;> [exact .pure fun hb => h (by simpa using hb); skip]
+  refine .pureBind <| (isDefEqUnitLike.WF c1 d1).bind fun _ _ _ h => ?_
+  split <;> [exact .pure fun _ => h ‹_›; skip]
+  exact .pureBind <| .pure nofun
